Played some more with the example.

cptd-ssr/cpdt-chapter8.v
@@ -21,25 +21,38 @@ Inductive exp : type -> Set :=
 *)
 
 Inductive exp t := 
-  NConst' of nat & Nat = t
-| Plus' of exp Nat & exp Nat & Nat = t
-| Eq' of exp Nat & exp Nat & Bool = t
-| BConst' of bool & Bool = t
-| And' of exp Bool & exp Bool & Bool = t
-| If' of exp Bool & exp t & exp t
-| Pair' t1 t2 of exp t1 & exp t2 & Prod t1 t2 = t
-| Fst' t1 t2 of exp (Prod t1 t2) & t1 = t
-| Snd' t1 t2 of exp (Prod t1 t2) & t2 = t.
+  NConst' of Nat = t & nat
+| Plus' of Nat = t & exp Nat & exp Nat
+| Eq' of  Bool = t & exp Nat & exp Nat
+| BConst' of Bool = t & bool 
+| And' of Bool = t & exp Bool & exp Bool 
+| If of exp Bool & exp t & exp t
+| Pair' t1 t2 of Prod t1 t2 = t & exp t1 & exp t2 
+| Fst t2 of exp (Prod t t2)
+| Snd t1 of exp (Prod t1 t).
 
-Definition NConst n := NConst' n (erefl _).
-Definition Plus e1 e2 := Plus' e1 e2 (erefl _).
-Definition Eq e1 e2 := Eq' e1 e2 (erefl _).
-Definition BConst n := BConst' n (erefl _).
-Definition And e1 e2 := And' e1 e2 (erefl _).
-Definition If b e1 e2 := @If' b e1 e2.
-Definition Pair t1 t2 e1 e2 := @Pair' _ t1 t2 e1 e2 (erefl _).
-Definition Fst t1 t2 e := @Fst' _ t1 t2 e (erefl _).
-Definition Snd t1 t2 e := @Snd' _ t1 t2 e (erefl _).
+Notation NConst := (NConst' (erefl _)).
+Notation Plus := (Plus' (erefl _)).
+Notation Eq := (Eq' (erefl _)).
+Notation BConst := (BConst' (erefl _)).
+Notation And := (And' (erefl _)).
+Notation Pair := (Pair' (erefl _)).
+
+(* a better induction principle, to gather the like constructors *)
+(* and remove unnecessary type equations *)
+
+Lemma exp_ind' (P : forall t : type, exp t -> Prop) : 
+        [/\ forall n, P Nat (NConst n) &
+            forall b, P Bool (BConst b)] ->
+        [/\ forall e1 e2, P Nat e1 -> P Nat e2 -> P Nat (Plus e1 e2),
+            forall e1 e2, P Nat e1 -> P Nat e2 -> P Bool (Eq e1 e2) &
+            forall e1 e2, P Bool e1 -> P Bool e2 -> P Bool (And e1 e2)] ->
+        (forall t e e1 e2, P Bool e -> P t e1 -> P t e2 -> P t (If e e1 e2)) ->
+        (forall t1 t2 e1 e2, P t1 e1 -> P t2 e2 -> P (Prod t1 t2) (Pair e1 e2)) ->
+        [/\ forall t1 t2 e, P (Prod t1 t2) e -> P t1 (Fst e) &
+            forall t1 t2 e, P (Prod t1 t2) e -> P t2 (Snd e)] ->
+        forall t e, P t e.
+Proof. by case=>?? [???] ?? [??] t; elim=>t' *; try subst t'; intuition. Qed.
 
 Definition cast T (t t' : type) (r : t = t') (e : T t) :=
   match r in (_ = t') return T t' with erefl => e end.
@@ -48,6 +61,7 @@ Definition cast T (t t' : type) (r : t = t') (e : T t) :=
 Lemma eqc T t (r : t = t) (e : T t) : cast r e = e.
 Proof. by move: r; apply: Streicher_K. Qed.
 
+(*
 (* re-introducing casts *)
 Lemma recast T t t' (P : forall t, t' = t -> T t) (r : t' = t) : 
         P t r = cast r (P t' (erefl _)).
@@ -71,40 +85,79 @@ Inductive exp_spec t : exp t -> Type :=
 | snd_exp t1 (e : exp (Prod t1 t)) : exp_spec (Snd e).
 
 Lemma expP t (e : exp t) : exp_spec e.
-Proof. 
-by case: e=>*; rewrite 1?(recast (fun t => _)); try subst t; constructor.
-Qed.
+Proof. case: e=>*. rewrite 1?(recast (fun t => _)); constructor. Qed.
 
 (* test goal *)
 Lemma xx n (x : exp Nat) : x = NConst n.
 Proof. case/expP: x=>//. Abort.
-
+*)
 
 Fixpoint typeDenote (t : type) : Set :=
   match t with
-    | Nat => nat
-    | Bool => bool
-    | Prod t1 t2 => prod (typeDenote t1) (typeDenote t2)
+    Nat => nat
+  | Bool => bool
+  | Prod t1 t2 => prod (typeDenote t1) (typeDenote t2)
   end.
-
-(*
-Definition cast t t' (r : t = t') (e : typeDenote t) :=
-  match r in (_ = t') return typeDenote t' with erefl => e end.
-*)
 
 Fixpoint expDenote t (e : exp t) : typeDenote t :=
   match e with
-  | NConst' n r => cast r n
-  | Plus' e1 e2 r => cast r (expDenote e1 + expDenote e2)
-  | Eq' e1 e2 r => cast r (expDenote e1 == expDenote e2) 
-  | BConst' b r => cast r b
-  | And' e1 e2 r => cast r (expDenote e1 && expDenote e2)
-  | If' e' e1 e2 => if expDenote e' then expDenote e1 else expDenote e2
-  | Pair' t1 t2 e1 e2 r => cast r (expDenote e1, expDenote e2)
-  | Fst' _ _ e' r => cast r (fst (expDenote e'))
-  | Snd' _ _ e' r => cast r (snd (expDenote e'))
+    NConst' r n => cast r n
+  | Plus' r e1 e2 => cast r (expDenote e1 + expDenote e2)
+  | Eq' r e1 e2 => cast r (expDenote e1 == expDenote e2) 
+  | BConst' r b => cast r b
+  | And' r e1 e2 => cast r (expDenote e1 && expDenote e2)
+  | If e' e1 e2 => if expDenote e' then expDenote e1 else expDenote e2
+  | Pair' _ _ r e1 e2 => cast r (expDenote e1, expDenote e2)
+  | Fst _ e' => fst (expDenote e')
+  | Snd _ e' => snd (expDenote e')
   end.
 
+Lemma fst_out t1 t2 s1 s2 : Prod t1 t2 = Prod s1 s2 -> t1 = s1.
+Proof. by case. Defined.
+
+Lemma snd_out t1 t2 s1 s2 : Prod t1 t2 = Prod s1 s2 -> t2 = s2.
+Proof. by case. Qed.
+
+Fixpoint cfold t (e : exp t) : exp t :=
+  match e with
+    NConst' r n => NConst' r n
+  | Plus' r e1 e2 => 
+      let: (e1', e2') := (cfold e1, cfold e2) in
+      if (e1', e2') is (NConst' _ n1, NConst' _ n2) then NConst' r (n1 + n2)
+      else Plus' r e1' e2'
+  | Eq' r e1 e2 =>
+      let: (e1', e2') := (cfold e1, cfold e2) in
+      if (e1', e2') is (NConst' _ n1, NConst' _ n2) then BConst' r (n1 == n2) 
+      else Eq' r e1' e2' 
+  | BConst' r b => BConst' r b
+  | And' r e1 e2 =>
+      let: (e1', e2') := (cfold e1, cfold e2) in
+      if (e1', e2') is (BConst' _ b1, BConst' _ b2) then BConst' r (b1 && b2)
+      else And' r e1' e2' 
+  | If e e1 e2 =>
+      let: e' := cfold e in
+      match e' with
+        BConst' _ true => cfold e1
+      | BConst' _ false => cfold e2
+      | _ => If e' (cfold e1) (cfold e2)
+      end
+  | Pair' _ _ r e1 e2 => Pair' r (cfold e1) (cfold e2) 
+  | Fst _ e =>
+      let: e' := cfold e in
+      if e' is Pair' _ _ r e1 e2 then cast (fst_out r) e1 else Fst e'
+  | Snd _ e =>
+      let e' := cfold e in
+      if e' is Pair' _ _ r e1 e2 then cast (snd_out r) e2 else Snd e'
+  end. 
+
+Lemma cfold_correct t (e : exp t) : expDenote e = expDenote (cfold e).
+Proof.
+elim/exp_ind': e=>//=.
+- by split=>?? ->->; do 2![case: (cfold _)=>//= *]; rewrite !eqc. 
+- by move=>???? ->->->; case: (cfold _)=>//= *; rewrite eqc; case: ifP.
+- by move=>???? ->->.
+by split=>??? ->; case: (cfold _)=>//= ?? r; case: r (r)=>->-> *; rewrite !eqc.
+Qed.
 
 
 
